\documentclass[12pt,letterpaper]{article}

\usepackage{graphicx,amssymb,amsmath,bm,color,multicol}
\usepackage{../newcommand}
\sloppy
\newcommand{\ignore}[1]{}

\newenvironment{proof}{\noindent{\bf Proof:}}{\qed\bigskip}

\newtheorem{theorem}{Theorem}
\newtheorem{corollary}{Corollary}
\newtheorem{lemma}{Lemma} 
\newtheorem{claim}{Claim}
\newtheorem{fact}{Fact}
\newtheorem{definition}{Definition}
\newtheorem{assumption}{Assumption}
\newtheorem{observation}{Observation}
\newtheorem{example}{Example}
\newcommand{\qed}{\rule{7pt}{7pt}}

\usepackage{times}
\usepackage{ulem}
\usepackage[nocenter]{qtree}
\usepackage{tree-dvips}
\usepackage{gb4e}

\newcommand{\homework}[4]{
	\thispagestyle{plain} 
	\newpage
	\setcounter{page}{1}
	\noindent
	\begin{center}
		\framebox{ \vbox{ \hbox to 6.28in
				{\bf ECON 4190: Industrial Organization \hfill #1} %change course name
				\vspace{4mm}
				\hbox to 6.28in
				{\hspace{2.5in}\large\mbox{Homework #2}}
				\vspace{4mm}
				\hbox to 6.28in
				{{\it Collaborators: #3\hfill}}
			}}
		\end{center}
	}

\oddsidemargin 0in
\evensidemargin 0in
\textwidth 6.5in
\topmargin -0.5in
\textheight 9.0in

\begin{document}

% Modify this command to be your name and computing ID
\homework{Fall 2021}{$5$}{Alex Shen (as5gd), Sean Velhagen (spv5hq), Max Bresticker (mtb9sex)}

Pledge: On my honor, I pledge that I have neither given nor received help on this assignment 
Signature: \textit{Alex Shen, Sean Velhagen, Max Bresticker}

\begin{enumerate}
	
\item[3.2)] 

\item[4.1)]
\begin{enumerate}
    \item[1.] We start off by maximizing Firm 1's profit:
    \begin{align*}
        max_{p_1} \pi_1 &= (a-2p_1 + p_2)(p_1 - 0) \\
        \frac{\partial \pi_1}{\partial p_1} &= a - 4p_1 + p_2 = 0 \\
        \therefore p_1 &= \frac{a + p_2}{4}
    \end{align*} 
    Then, maximize Firm 2's profit to solve for $p_2$, and then plug in $p_1$ to solve for both:
    \begin{align*}
        max_{p_2} \pi_2 &= (a-2p_2 + p_1)(p_2 - c) \\
        \frac{\partial \pi_2}{\partial p_2} &= (a - 2p_2 + p_1) + (p_2 - c)(-2) = 0 \\
        0 &= a - 2p_2 + p_1 - 2p_2 + 2c \\
        \therefore p_2 &= \frac{p_1 + a + 2c}{4} = \frac{\frac{a + p_2}{4} + a + 2c}{4} \\
        16p_2 &= a + p_2 + 4a + 8c \\
        \therefore p_2 &= \frac{5a + 8c}{15} \\
        \therefore p_1 &= \frac{5 + 2a}{15}
    \end{align*} 
    \item[2.] 
    \item[3.] 
\end{enumerate}

\item[4.3)] 

\begin{enumerate}
    \item[1.] The game tree here can be (roughly) visualized as follows:

    \includegraphics[scale=0.15]{game-tree.jpg}
                                          
    In scenarios where Firm 2 discloses its cost, Firm 1's response is very simple - when $c_2 = 0$, the firms have equal costs and will thus reach the Cournot equilibrium outcome, where $q_1 = q_2 = \frac{1}{3}$, and $\pi_1 = \pi_2 = (1-q -q)* q= \frac{1}{9}$. If $c_2$ is prohibitively high, then Firm 1 will simply act as a monopolist, producing $q=\frac{1}{2}$ with a profit of $\frac{1}{4}$, whereas Firm 2 will have a quantity produced and profit of 0.
    
    When Firm 2 doesn't disclose its cost, Firm 1 can only maximize its profit function using an expected value for $q_2$. Since the probability of both cases is $p=0.5$, $E(p_2)$ can be determined simply by halving the quantity Firm 2 produces in the Cournot equilibrium, so $E(q_2) = \frac{1-q_1}{2} * \frac{1}{2} = \frac{1-q_1}{4}$. Given this value, we can simply derive Firm 1's best response as follows by maximizing their expected profit:
    
    \begin{align*}
        max_{q_1} E(\pi_1) &= (1 - q_1 - E(q_2)) * (q_1) \\
        \frac{\partial E(\pi_1)}{\partial q_1} &= 1 - 2q_1 - E(q_2) = 0 \\
        \therefore q_1^* &= \frac{1 - E(q_2)}{2} \\
        &= \frac{1}{2} * (1 - \frac{1-q_1}{4}) \\
        8q_1 &= 4 - 1 + q_1 \\
        q_1 &= \frac{3}{7} \\
        \therefore q_2 &= \frac{2}{7}
    \end{align*}
    
    With these quantities, we can easily determine the profits to be $\pi_1 = (1 - \frac{3}{7} - \frac{2}{2*7}) * \frac{3}{7} = \frac{9}{49}$ (plugging back into our expected value function) and $\pi_2 = (1 - \frac{3}{7} - \frac{2}{7}) * \frac{2}{7} = \frac{4}{49}$ (since Firm 1 is always in the market, Firm 2 doesn't need to use expected values).
    
    {\color{blue}\textbf{Solution:} With information sharing, the outcome will either resemble that of Cournot duopoly if $c_2=0$ or monopoly by Firm 1 if $c_2$ is prohibitively high. Without information sharing, the equilibrium is $q_1  = \frac{3}{7}, q_2 = \frac{2}{7}, \pi_1 = \frac{9}{49}, \pi_2 = \frac{4}{49}$}

    \item[2.] If $c_2$ is prohibitively high, then Firm 2 doesn't care about sharing its information because its profit is 0 either way. Otherwise, if $c_2 = 0$, Firm 2 has an incentive to share its cost as $\frac{1}{9} > \frac{4}{49}$ i.e. their profit is higher in the Cournot duopoly equilibrium than the non-sharing equilibrium. 
    \item[3.] If Firm 2 shares information, then Firm 1's expected profit is $\frac{1}{2} (\frac{1}{4} + \frac{1}{9}) = \frac{13}{72}$. This is less than the expected profit of $\frac{9}{49}$s when information is not shared, so Firm 1 is worse off in information sharing.
\end{enumerate}

\item[4)]

\begin{enumerate}

    \item In general, the profit function for a monopoly (colluding firms) is as follows:
    \begin{align*}
        \pi^m &= P(Q)Q - c(Q)
    \end{align*}
    
    In this case, $P(Q) = a-bQ$ and $c(Q) = cQ$, so:
    \begin{align*}
        \pi^m &= (a-bQ)Q - cQ\\
        FOC_{wrt.Q}: 0 &= a-2bQ^m - c\\
        Q^m &= \frac{a-c}{2b}
    \end{align*}
    
    Firm i's profit function in a 2-firm Cournot model with the given inverse demand and cost function is as follows:
    \begin{align*}
        \pi_i &= (a - b(q_1 + q_2))q_i - cq_i
    \end{align*}
    
    So, the firms' profit functions are as follows:
    \begin{align*}
        \pi_1 &= (a - b(q_1 + q_2))q_1 - cq_1\\
        \pi_2 &= (a - b(q_1 + q_2))q_2 - cq_2
    \end{align*}
    
    It is easily seen here that optimizing firm 1's profits will give a similar expression to optimizing firm 2's profits, just with $q_1$ and $q_2$ interchanged. Let us optimize firm 1:
    \begin{align*}
        FOC_{wrt.q_1}: 0 &= -bq_1^c + (a-b(q_1^c + q_2)) - c\\
        0 &= a - 2bq_1^c - bq_2 - c\\
        q_1^c &= \frac{a - bq_2 - c}{2b}
    \end{align*}
    
    We may interchange $q_1$ and $q_2$ to find $q_2^c$:
    \begin{align*}
        q_2^c &= \frac{a - bq_1 - c}{2b}
    \end{align*}
    
    To find the Cournot equilibrium, we can plug in firm 2's best response  function into firm 1's best response function and solve for $q_1^c$ as a function of constants. Again, we see here that the process for solving for $q_1^c$ as a function of constants is similar to the process for solving for $q_2^c$ as a function of constants, just with $q_1^c$ and $q_2^c$ flipped. Plugging $q_2^c$ into firm 1's best response function, we have:
    \begin{align*}
        q_1^c &= \frac{a - b(\frac{a - bq_1^c - c}{2b}) - c}{2b}\\
        q_1^c &= \frac{a}{2b} - \frac{a}{4b} + \frac{q_1^c}{4} + \frac{c}{4b} - \frac{c}{2b}\\
        \frac{3}{4}q_1^c &= \frac{a}{4b} - \frac{c}{4b}\\
        q_1^c &= \frac{a-c}{3b}
    \end{align*}
    
    We may interchange $q_1^c$ and $q_2^c$ to find $q_2^c$ as a function of constants:
    \begin{align*}
        q_2^c &= \frac{a-c}{3b}\\
        Q &= q_1 + q_2\\
        Q^c &= q_1^c + q_2^c\\
        Q^c &= \frac{2(a-c)}{3b}\\
        Q^m &= \frac{a-c}{2b}\\
        \frac{2(a-c)}{3b} &> \frac{a-c}{2b}\\
        Q^c &> Q^m \ \blacksquare
    \end{align*}
    
    \item 
    
    \item $MC(q_i) = cq_i$, so the profit function for firm i is as follows:
    \begin{align*}
        \pi_i &= (a - b(q_1 + q_2))q_i - \frac{cq_i^2}{2}
    \end{align*}
    
    We can find $q_1^c$ and $q_2^c$ using the same techniques that we used in 4.a:
    \begin{align*}
        \pi_1 &= (a - b(q_1 + q_2))q_1 - \frac{cq_1^2}{2}\\
        FOC_{wrt.q_1}: 0 &= -bq_1^c + (a-b(q_1^c + q_2)) - cq_1^c\\
        0 &= a - (2b + c)q_1^c - bq_2\\
        q_1^c &= \frac{a - bq_2}{2b + c}
    \end{align*}
    
    By symmetry, we have:
    \begin{align*}
        q_2^c &= \frac{a - bq_1^c}{2b + c}
    \end{align*}
    
    Again, we plug $q_2^c$ into $q_1^c$ to get $q_1^c$ as a function of constants:
    \begin{align*}
        q_1^c &= \frac{a - b(\frac{a - bq_1^c}{2b + c})}{2b + c}\\
        q_1^c &= \frac{a}{2b+c} - \frac{ab}{(2b+c)^2} + \frac{b^2q_1^c}{(2b+c)^2}\\
        (1-\frac{b^2}{(2b+c)^2})q_1^c &= \frac{a(b+c)}{(2b+c)^2}\\
        ((2b+c)^2 - b^2)q_1^c &= a(b+c)\\
        q_1^c &= \frac{a(b+c)}{3b^2 + 4bc + c^2}
    \end{align*}
    
    By symmetry, we have:
    \begin{align*}
        q_2^c &= \frac{a(b+c)}{3b^2 + 4bc + c^2}\\
        Q^c &= q_1^c + q_2^c\\
        \therefore Q^c &= \frac{2a(b+c)}{3b^2 + 4bc + c^2}
    \end{align*}
    
    \item Now that $c_1$ isn't necessarily equal to $c_2$, the monopoly (collusion) profit function is as follows:
    \begin{align*}
        \pi^m &= (a-b(q_1 + q_2))(q_1 + q_2) - (c_1q_1 + c_2q_2)
    \end{align*}

\end{enumerate}


\end{enumerate}
	
\end{document}
